Fix an error in traceRuleOnPiece_rel .

core/Semantics.v
@@ -33,6 +33,16 @@ Definition allTuples (tr: Transformation) (sm : SourceModel) : list InputPiece :
 Definition isTuple (sm : SourceModel) ip : Prop := 
   List.incl ip sm.(modelElements).
 
+Lemma p1 : forall tr sm ip,
+  List.In ip (allTuples tr sm) -> isTuple sm ip.
+Proof.
+  unfold allTuples.
+  unfold isTuple.
+
+  intros ; eapply TupleUtils.tuples_up_to_n_incl ; eassumption.
+Qed. 
+
+
 (* executable *)
 Definition matchingRules (tr: Transformation) (sm : SourceModel) (sp: InputPiece) : list Rule :=
   List.filter (fun (r:Rule) => evalGuard r sm sp) tr.(rules).
@@ -40,6 +50,20 @@ Definition matchingRules (tr: Transformation) (sm : SourceModel) (sp: InputPiece
 (* predicative *)
 Definition matchingRule (tr: Transformation) (sm : SourceModel) (sp: InputPiece) r : Prop :=
     List.In r tr.(rules) /\ UserExpressions.guard_ok r sm sp.
+
+Lemma p2 :
+ forall tr sm sp r,
+   List.In r (matchingRules tr sm sp) <-> matchingRule tr sm sp r.
+Proof.
+  unfold matchingRules.
+  unfold matchingRule.
+  Search (In _ (filter _ _)).
+  setoid_rewrite filter_In.
+  unfold guard_ok.
+  unfold evalGuard.
+  tauto.
+Qed.
+
 
 (** * Building traces *)
 
@@ -56,13 +80,32 @@ Definition traceElementOnPiece (o: OutputPatternUnit) (sm: SourceModel) (sp: Inp
 (* predicatif *)
 Inductive traceElementOnPiece_rel (o: OutputPatternUnit) (sm: SourceModel) (sp: InputPiece) (iter: nat)
   : TraceLink -> Prop :=
-    | r1 : forall v, evalOutputPatternUnit_rel o sm sp iter v ->
-  traceElementOnPiece_rel o sm sp iter
-     {| 
-        source := (sp, iter, o.(opu_name)) ;
-        produced := v ;
-        linkPattern := o.(opu_link) 
-      |}.
+    | r1 : 
+      forall v, 
+        evalOutputPatternUnit_rel o sm sp iter v ->
+        traceElementOnPiece_rel o sm sp iter
+         {| 
+           source := (sp, iter, o.(opu_name)) ;
+            produced := v ;
+            linkPattern := o.(opu_link) 
+          |}.
+
+Lemma p3 : 
+  forall o sm sp it tl,
+  traceElementOnPiece_rel o sm sp it tl <-> traceElementOnPiece o sm sp it = Some tl.
+Proof.
+  unfold traceElementOnPiece.
+  intros ; split.
+  + intro H.
+    inversion_clear H.
+    unfold evalOutputPatternUnit_rel in H0.
+    unfold evalOutputPatternUnit.
+    rewrite H0.
+    reflexivity.
+  + intro H ; OptionUtils.monadInv H.
+    constructor.
+    exact H.
+Qed.
 
 (* executable *)
 Definition traceIterationOnPiece (r: Rule) (sm: SourceModel) (sp: InputPiece) (iter: nat) :  Trace :=
@@ -77,6 +120,23 @@ Inductive traceIterationOnPiece_rel (r: Rule) (sm: SourceModel) (sp: InputPiece)
         traceElementOnPiece_rel o sm sp iter tl -> 
       traceIterationOnPiece_rel r sm sp iter tl.
 
+Lemma p4 : forall r sm sp it tlk, 
+  traceIterationOnPiece_rel r sm sp it tlk <-> List.In tlk (traceIterationOnPiece r sm sp it).
+Proof.
+  unfold traceIterationOnPiece.
+  Search (In _ (flat_map _ _)).
+  setoid_rewrite in_flat_map.
+  Search (In _ (optionToList _)).
+  setoid_rewrite in_optionToList.
+  setoid_rewrite <- p3.
+  intros ; split ; intro H. 
+  + inversion_clear H.
+    eauto.
+  + destruct H as (o & H1 & H2).
+    econstructor ; eauto.
+Qed.
+
+
 (* executable *)
 Definition traceRuleOnPiece (r: Rule) (sm: SourceModel) (sp: InputPiece) : Trace :=
   flat_map 
@@ -84,12 +144,35 @@ Definition traceRuleOnPiece (r: Rule) (sm: SourceModel) (sp: InputPiece) : Trace
     (seq 0 (evalIterator r sm sp)).
 
 (* predicatif *)
-Inductive traceRuleOnPiece_rel (r: Rule) (sm: SourceModel) (sp: InputPiece) (tl:TraceLink) : Prop :=
+Inductive traceRuleOnPiece_rel (r: Rule) (sm: SourceModel) (sp: InputPiece) (tlk:TraceLink) : Prop :=
   | r3 : 
-    forall it, 
-    evalIterator_rel r sm sp it ->
-    traceIterationOnPiece_rel r sm sp it tl ->
-    traceRuleOnPiece_rel r sm sp tl.
+    forall nb_it current_it, 
+       current_it < nb_it -> 
+       evalIterator_rel r sm sp nb_it ->
+       traceIterationOnPiece_rel r sm sp current_it tlk ->
+       traceRuleOnPiece_rel r sm sp tlk.
+
+Lemma p5 : forall r sm sp tlk, 
+  traceRuleOnPiece_rel r sm sp tlk <-> List.In tlk (traceRuleOnPiece r sm sp).
+Proof.
+  unfold traceRuleOnPiece.
+  setoid_rewrite in_flat_map.
+  setoid_rewrite <- p4.
+  intros ; split ; intro H.
+  + inversion_clear H. 
+    apply UserExpressions.p1 in H1.
+    rewrite H1.
+    exists current_it ; split ; [ | auto].
+    Search (In _ (seq _ _)).
+    apply in_seq.
+    simpl.
+    Lia.lia.
+  + destruct H as (current_it & H1 & H2).
+    econstructor ; [ | apply UserExpressions.c1 | exact H2].
+    apply in_seq in H1.  
+    simpl in H1.
+    Lia.lia.
+Qed.
 
 (* executable *)
 Definition traceTrOnPiece (tr: Transformation) (sm : SourceModel) (sp: InputPiece) : Trace :=
@@ -131,7 +214,7 @@ Definition apply_link_pattern (tls:Trace) sm lk :list TargetLinkType :=
 
  (* predicative *)
 Definition apply_link_pattern_rel tls sm lk tl : Prop := 
-   List.In tl (lk.(linkPattern) (drop tls) (getIteration lk) sm (getSourcePiece lk) lk.(produced)).
+   List.In tl (lk.(linkPattern) (* fixme *) (drop tls) (getIteration lk) sm (getSourcePiece lk) lk.(produced)).
   
 
 (* executable *)
